finish ImplModelDealloc

disk-betree/ImplModelDealloc.i.dfy
@@ -20,7 +20,7 @@ module ImplModelDealloc {
     && forall r | r in IIndirectionTable(s.ephemeralIndirectionTable).graph :: ref !in IIndirectionTable(s.ephemeralIndirectionTable).graph[r]
   }
 
-  function Dealloc(k: Constants, s: Variables, io: IO, ref: BT.G.Reference)
+  function {:opaque} Dealloc(k: Constants, s: Variables, io: IO, ref: BT.G.Reference)
   : (res : (Variables, IO))
   requires Inv(k, s)
   requires io.IOInit?
@@ -52,6 +52,7 @@ module ImplModelDealloc {
       && WFVars(s')
       &&  M.Next(Ik(k), IVars(s), IVars(s'), UI.NoOp, diskOp(io'))
   {
+    reveal_Dealloc();
     var (s', io') := Dealloc(k, s, io, ref);
 
     if (
@@ -77,36 +78,76 @@ module ImplModelDealloc {
     // assert M.NextStep(Ik(k), IVars(s), IVars(s'), UI.NoOp, io.diskOp(), M.Step(BBC.BlockCacheMoveStep(BC.UnallocStep(ref))));
   }
 
-  /*
-  method FindDeallocable(s: Variables) returns (ref: Option<Reference>)
+  function FindDeallocableIterate(s: Variables, ephemeralRefs: seq<BT.G.Reference>, i: uint64)
+  : (ref: Option<Reference>)
+  requires 0 <= i as int <= |ephemeralRefs|
+  requires |ephemeralRefs| < 0x1_0000_0000_0000_0000;
+  decreases 0x1_0000_0000_0000_0000 - i as int
+  {
+    if i == |ephemeralRefs| as uint64 then (
+      None
+    ) else (
+      var ref := ephemeralRefs[i];
+      var isDeallocable := deallocable(s, ref);
+      if isDeallocable then (
+        Some(ref)
+      ) else (
+        FindDeallocableIterate(s, ephemeralRefs, i + 1)
+      )
+    )
+  }
+
+  function {:opaque} FindDeallocable(s: Variables)
+  : (ref: Option<Reference>)
   requires WFVars(s)
   requires s.Ready?
-  ensures ref.Some? ==> ref.value in IIndirectionTable(s.ephemeralIndirectionTable).graph
-  ensures ref.Some? ==> deallocable(s, ref.value)
-  ensures ref.None? ==> forall r | r in IIndirectionTable(s.ephemeralIndirectionTable).graph :: !deallocable(s, r)
   {
     // TODO once we have an lba freelist, rewrite this to avoid extracting a `map` from `s.ephemeralIndirectionTable`
-    var ephemeralTable := s.ephemeralIndirectionTable.ToMap();
-    var ephemeralRefs := SetToSeq(ephemeralTable.Keys);
+    var ephemeralRefs := setToSeq(s.ephemeralIndirectionTable.Keys);
 
     assume |ephemeralRefs| < 0x1_0000_0000_0000_0000;
 
-    var i: uint64 := 0;
-    while i as int < |ephemeralRefs|
-    invariant i as int <= |ephemeralRefs|
-    invariant forall k : nat | k < i as nat :: (
+    FindDeallocableIterate(s, ephemeralRefs, 0)
+  }
+
+  lemma FindDeallocableIterateCorrect(s: Variables, ephemeralRefs: seq<BT.G.Reference>, i: uint64)
+  requires 0 <= i as int <= |ephemeralRefs|
+  requires |ephemeralRefs| < 0x1_0000_0000_0000_0000;
+  requires s.Ready?
+  requires ephemeralRefs == setToSeq(s.ephemeralIndirectionTable.Keys)
+  requires forall k : nat | k < i as nat :: (
         && ephemeralRefs[k] in IIndirectionTable(s.ephemeralIndirectionTable).graph
         && !deallocable(s, ephemeralRefs[k]))
-    {
+  ensures var ref := FindDeallocableIterate(s, ephemeralRefs, i);
+      && (ref.Some? ==> ref.value in IIndirectionTable(s.ephemeralIndirectionTable).graph)
+      && (ref.Some? ==> deallocable(s, ref.value))
+      && (ref.None? ==> forall r | r in IIndirectionTable(s.ephemeralIndirectionTable).graph :: !deallocable(s, r))
+  decreases 0x1_0000_0000_0000_0000 - i as int
+  {
+    if i == |ephemeralRefs| as uint64 {
+      assert forall r | r in IIndirectionTable(s.ephemeralIndirectionTable).graph :: !deallocable(s, r);
+    } else {
       var ref := ephemeralRefs[i];
-      var isDeallocable := Deallocable(s, ref);
+      var isDeallocable := deallocable(s, ref);
       if isDeallocable {
-        return Some(ref);
+      } else {
+        FindDeallocableIterateCorrect(s, ephemeralRefs, i + 1);
       }
-      i := i + 1;
     }
-    assert forall r | r in IIndirectionTable(s.ephemeralIndirectionTable).graph :: !deallocable(s, r);
-    return None;
   }
-  */
+
+  lemma FindDeallocableCorrect(s: Variables)
+  requires WFVars(s)
+  requires s.Ready?
+  ensures var ref := FindDeallocable(s);
+      && (ref.Some? ==> ref.value in IIndirectionTable(s.ephemeralIndirectionTable).graph)
+      && (ref.Some? ==> deallocable(s, ref.value))
+      && (ref.None? ==> forall r | r in IIndirectionTable(s.ephemeralIndirectionTable).graph :: !deallocable(s, r))
+  {
+    reveal_FindDeallocable();
+    var ephemeralRefs := setToSeq(s.ephemeralIndirectionTable.Keys);
+    assume |ephemeralRefs| < 0x1_0000_0000_0000_0000;
+    FindDeallocableIterateCorrect(s, ephemeralRefs, 0);
+  }
+
 }
